tidying up pure encoding, much cleaner

examples/layeredeffects/ID3.fst
@@ -1,143 +1,60 @@
 module ID3
 
-val m (a : Type u#a) : Type u#a
-let m a = a
-
-val m_return (#a : Type) : a -> m a
-let m_return x = x
-
-val m_bind (#a #b : Type) : m a -> (a -> m b) -> m b
-let m_bind v f = f v 
-
-// w is an ordered (w_ord) monad with conjunction (w_conj) and actions from prop (w_act_prop)
+// The base type of WPs
 val w0 (a : Type u#a) : Type u#(max 1 a)
 let w0 a = (a -> Type0) -> Type0
 
+// We require monotonicity of them
 let monotonic (w:w0 'a) =
   forall p1 p2. (forall x. p1 x ==> p2 x) ==> w p1 ==> w p2
 
 val w (a : Type u#a) : Type u#(max 1 a)
 let w a = w:(w0 a){monotonic w}
 
-val w_ord (#a : Type) : w a -> w a -> Type0
-let w_ord wp1 wp2 = forall p. wp1 p ==> wp2 p
+let repr (a : Type) (wp : w a) : Type =
+  v:a{forall p. wp p ==> p v}
 
-val w_ord_trans (#a : Type) (wp1 : w a) (wp2 : w a) (wp3 : w a) : Lemma (requires w_ord wp1 wp2 /\ w_ord wp2 wp3) (ensures w_ord wp1 wp3)
-let w_ord_trans wp1 wp2 wp3 = ()
+let return (a : Type) (x : a) : repr a (fun p -> p x) =
+  x
 
-// GM: this is "assume"
-val w_act_prop (#a : Type) : Type0 -> w a -> w a
-let w_act_prop phi wp = fun p -> phi ==> wp p
+let bind (a b : Type) (wp_v : w a) (wp_f: a -> w b)
+    (v : repr a wp_v)
+    (f : (x:a -> repr b (wp_f x)))
+: repr b (fun p -> wp_v (fun x -> wp_f x p))
+= f v
 
-val w_conj (#a : Type) : w a -> w a -> w a
-let w_conj wp1 wp2 p = wp1 p /\ wp2 p
+let subcomp (a:Type) (wp1 wp2: w a)
+    (f : repr a wp1)
+: Pure (repr a wp2)
+       (requires (forall p. wp2 p ==> wp1 p))
+       (ensures fun _ -> True)
+= f
 
-val w_return (#a : Type) : a -> w a
-let w_return x = fun p -> p x
-
-val w_bind (#a #b : Type) : w a -> (a -> w b) -> w b
-let w_bind wp1 k = fun p -> wp1 (fun x -> k x p)
-
-val w_bind_monotonic (#a #b : Type) (m1 : w a) (m2 : w a) (f1 : a -> w b) (f2 : a -> w b) : Lemma (requires w_ord m1 m2 /\ (forall (a : a).{:pattern f2 a} w_ord (f1 a) (f2 a))) (ensures w_ord (w_bind m1 f1) (w_bind m2 f2))
-let w_bind_monotonic m1 m2 f1 f2 = ()
-
-// we can define an "equality" on w a
-val w_equiv (#a : Type) : w a -> w a -> Type0
-let w_equiv wp1 wp2 = w_ord wp1 wp2 /\ w_ord wp2 wp1
-
-// the monad morphism that connect the two monadic structures
-val interp (#a : Type) : m a -> w a
-
-let interp #a (x:m a) = fun p -> p x
-
-val interp_ret (#a : Type) (x : a) : Lemma (interp (m_return x) `w_equiv` w_return x)
-let interp_ret x = ()
-
-let dro_w wp2 wp1 = w_ord wp1 wp2
-
-val interp_bind (#a #b : Type) (v : m a) (f : a -> m b) : Lemma (interp (m_bind v f) `w_equiv` w_bind (interp v) (fun a -> interp (f a)))
-let interp_bind v f = ()
-
-// In DM4A we would have something like:
-
-// total
-// reifiable
-// reflectable
-// new_effect {
-//   DM4A : a:Type -> Effect
-//   with
-//        repr      = m
-//      ; return    = m_return
-//      ; bind      = m_bind
-
-//      ; wp_type   = w
-//      ; return_wp = w_return
-//      ; bind_wp   = w_bind
-
-//      ; interp    = interp
-// }
-
-// In layered effects, we instead construct the Dijkstra monad as a
-// sigma type (see the paper)
-
-let dm (a : Type) (wp : w a) : Type =
-  c:(m a){wp `w_ord` interp c}
-
-let irepr (a : Type) (wp: w a) = dm a wp
-
-let ireturn (a : Type) (x : a) : irepr a (w_return x) =
- interp_ret x;
- m_return x
-
-let ibind (a b : Type) (wp_v : w a) (wp_f: a -> w b) (v : irepr a wp_v) (f : (x:a -> irepr b (wp_f x))) : irepr b (w_bind wp_v wp_f) =
-  m_bind v f
-
-let isubcomp (a:Type) (wp1 wp2: w a) (f : irepr a wp1) : Pure (irepr a wp2) (requires w_ord wp2 wp1) (ensures fun _ -> True) = f
-
-let wp_if_then_else (#a:Type) (wp1 wp2:w a) (p:Type0) : w a=
-  w_conj (w_act_prop p wp1) (w_act_prop (~p) wp2)
-
-let i_if_then_else (a : Type) (wp1 wp2 : w a) (f : irepr a wp1) (g : irepr a wp2) (p : Type0) : Type =
-  irepr a (wp_if_then_else wp1 wp2 p)
-
-module T = FStar.Tactics
-
-let lem_if_1 (#a:Type) (wp1 wp2 : w a) (p:Type0) (f : irepr a wp1) (g : irepr a wp2)
-  : Lemma (p ==> w_ord (wp_if_then_else wp1 wp2 p) wp1)
-          [SMTPat ()]
-          by (T.norm [delta])
-  = 
-  ()
-  
-let lem_if_2 (#a:Type) (wp1 wp2 : w a) (p:Type0) (f : irepr a wp1) (g : irepr a wp2)
-  : Lemma ((~p) ==> w_ord (wp_if_then_else wp1 wp2 p) wp2)
-          [SMTPat ()]
-          by (T.norm [delta])
-  = 
-  ()
+let if_then_else (a : Type) (wp1 wp2 : w a) (f : repr a wp1) (g : repr a wp2) (p : Type0) : Type =
+  repr a (fun post -> (p ==> wp1 post) /\ ((~p) ==> wp2 post))
 
 // requires to prove that
-// p  ==> subcomp f (if_then_else p f g)
-// ~p ==> subcomp g (if_then_else p f g)
-// that's what the hacky SMTPats are for, we don't have a way
-// to provide a proof explicitly
+// p  ==> f <: (if_then_else p f g)
+// ~p ==> g <: (if_then_else p f g)
+// if the effect definition fails, add lemmas for the
+// above with smtpats
 total
 reifiable
 reflectable
 layered_effect {
   ID : a:Type -> wp : w a -> Effect
-  with repr         = irepr;
-       return       = ireturn;
-       bind         = ibind;
-       subcomp      = isubcomp; 
-       if_then_else = i_if_then_else
+  with repr         = repr;
+       return       = return;
+       bind         = bind;
+       subcomp      = subcomp;
+       if_then_else = if_then_else
 }
 
 let lift_pure_nd (a:Type) (wp:pure_wp a{monotonic wp}) (f:(unit -> PURE a wp)) :
-  Pure (irepr a wp) (requires (wp (fun _ -> True)))
-                    (ensures (fun _ -> True))
-  = m_return (f ())
-
+  Pure (repr a wp) (requires (wp (fun _ -> True))) // Can only lift from `Tot`
+                   (ensures (fun _ -> True))
+  = f ()
+  
 sub_effect PURE ~> ID = lift_pure_nd
 
 (* Checking that it's kind of usable *)
@@ -145,22 +62,20 @@ sub_effect PURE ~> ID = lift_pure_nd
 val test_f : unit -> ID int (fun p -> p 5 /\ p 3)
 let test_f () = 3
 
-(* Need the compute sadly, not sure why *)
-let l () : Tot int =
-  let o = reify (test_f ()) in
-  o
+module T = FStar.Tactics
+
+let l () : int =
+  reify (test_f ())
 
 effect Id (a:Type) (pre:pure_pre) (post:pure_post' a pre) =
         ID a (fun (p:pure_post a) -> pre /\ (forall (pure_result:a). post pure_result ==> p pure_result))
 
 effect IdT (a:Type) = Id a True (fun _ -> True)
 
-#set-options "--debug ID --debug_level SMTQuery"
-
-(* Can't prove termination... why? And uncommenting the `explode`
- * actually makes F* explode :-) *)
-[@@expect_failure]
-let rec sum (l : list int) : IdT int //by (T.explode ())
+// Can't lift because of the strengthening, I believe. But can't we
+//prove it on the spot?
+[@@expect_failure [19]]
+let rec sum (l : list int) : IdT int
  =
   match l with
   | [] -> 0
